Proof of simulation Pallene -> Lir

pall2lir.v
@@ -66,6 +66,27 @@ Notation "'<' t1 '<=' t2 '>' e" := (Cast t1 t2 e)
     (at level 50, t1 at next level, t2 at next level).
 
 
+Lemma CastStep : forall t1 t2 e m e' m',
+  step m e m' e' ->
+  step m (<t1 <= t2> e) m' (<t1 <= t2> e').
+Proof.
+  intros * HSt.
+  unfold Cast.
+  destruct t1; destruct t2; eauto using step.
+  destruct (dec_Tag t t0); eauto using step.
+Qed.
+
+
+Lemma CongCast : forall t1 t2 e m e' m',
+  multistep m e m' e' ->
+  multistep m (<t1 <= t2> e) m' (<t1 <= t2> e').
+Proof.
+  intros * HSt.
+  induction HSt; eauto using multistep, CastStep.
+Qed.
+
+
+
 (*
 ** Get the ground type of an expression; if correctly typed;
 ** otherwise assume nil. (The expression will always be correctly
@@ -80,6 +101,10 @@ Definition tagOf Γ e : IRType :=
 
 Lemma tagOfT : forall Γ e T, typeOf Γ e = Some T -> tagOf Γ e = PT2IRT T.
 Proof. intros. unfold tagOf. rewrite H. trivial. Qed.
+
+
+Lemma tagOfT' : forall Γ e T, Γ |= e : T -> tagOf Γ e = PT2IRT T.
+Proof. eauto using tagOfT, typeOfCorrect'. Qed.
 
 
 Lemma tagStar2type : forall Γ e,
@@ -157,6 +182,14 @@ Ltac breakTagOf :=
   end.
 
 
+Lemma PT2IRTag : forall tg T,
+  PT2IRT T = Tag2Type tg -> T <> PTStar.
+Proof.
+  intros * Heq HCnt.
+  destruct T; discriminate.
+Qed.
+
+
 Lemma PTStarB : forall (T : PType),
     PT2IRT T = IRTStar -> T = PTStar.
 Proof.
@@ -188,10 +221,13 @@ Qed.
 (*
 ** Compilation of well-typed programs results in well-typed code
 *)
-Theorem Pall2LirWellTyped : forall Γ (e : PE) T,
-    Γ |= e : T -> IRTyping (TP2TGamma Γ) (Pall2Lir Γ e) (PT2IRT T).
+Theorem Pall2LirWellTyped : forall Γ Γ' (e : PE) T T',
+    Γ |= e : T ->
+    TP2TGamma Γ = Γ' ->
+    PT2IRT T = T' ->
+    IRTyping Γ' (Pall2Lir Γ e) T'.
 Proof with eauto using IRTyping.
-  intros Γ e T H.
+  intros * H Eq1 Eq2. subst.
   induction H; simpl in *;
   eauto using IRTyping,TP2TGammaIn;
   repeat match goal with
@@ -267,5 +303,590 @@ Proof with eauto using IRTyping.
   + unfold PT2IRT in *.
     trivial.
 Qed.
+
+
+Lemma typeOfEq : forall Γ1 e1 Γ2 e2 T,
+  Γ1 |= e1 : T ->
+  Γ2 |= e2 : T ->
+  typeOf Γ1 e1 = typeOf Γ2 e2.
+Proof.
+  intros * HTy1 HTy2.
+  erewrite typeOfCorrect'; eauto.
+  erewrite typeOfCorrect'; eauto.
+Qed.
+
+Lemma tagOfEq : forall Γ1 e1 Γ2 e2 T,
+  Γ1 |= e1 : T ->
+  Γ2 |= e2 : T ->
+  tagOf Γ1 e1 = tagOf Γ2 e2.
+Proof.
+  intros * HTy1 HTy2.
+  unfold tagOf.
+  erewrite typeOfEq; eauto.
+Qed.
+
+
+Ltac tagOf2T :=
+  repeat   (* replace tagOfs with theirs types *)
+      (erewrite tagOfT';
+       eauto using PTyping, PinclusionType, inclusion_update,
+                   Psubst_typing, inclusion_shadow, inclusion_permute,
+                   PexpPreservation).
+
+
+Lemma Pall2LirEEnv : forall Γ Γ' e T,
+  Γ |= e : T ->
+  inclusion Γ Γ' ->
+  Pall2Lir Γ e = Pall2Lir Γ' e.
+Proof.
+  intros * HTy HIn.
+  generalize dependent Γ'.
+  induction HTy; intros; subst; trivial;
+  simpl;   (* expose tagOfs *)
+  tagOf2T;
+  repeat match goal with   (* do the rewrites from the hypotheses *)
+  | [ H: _ -> _ -> _ = _ |- _] =>
+     erewrite H; eauto using inclusion_update; clear H
+  end.
+Qed.
+
+
+
+Lemma Psubst : forall Γ var Tvar e1 e2 te,
+  (var |=> Tvar; Γ) |= e2 : te ->
+  MEmpty |= e1 : Tvar ->
+  Pall2Lir Γ ([var := e1] e2) =
+    lir.substitution var (Pall2Lir MEmpty e1) (Pall2Lir (var |=> Tvar; Γ) e2).
+Proof.
+  intros * HTy2 HTy1.
+  generalize dependent te.
+  generalize dependent Γ.
+  induction e2; intros * HTy2; trivial; inversion HTy2; subst;
+  simpl;
+
+  repeat match goal with   (* do the rewrites from the hypotheses *)
+  | [ H: _ -> _ -> _ -> _ = _ |- _] =>
+     erewrite H; eauto using inclusion_update, PTyping; clear H
+  end.
+
+  - tagOf2T.
+    destruct (PT2IRT te); trivial.
+
+  - simpl.
+    tagOf2T.
+    destruct (PT2IRT T); trivial.
+
+  - simpl. destruct (string_dec var s); trivial.
+    symmetry. eauto using Pall2LirEEnv, PinclusionType, inclusion_empty.
+
+  - simpl.
+    tagOf2T.
+    destruct (PT2IRT te).
+    + destruct t; simpl; destruct (PT2IRT T1); trivial.
+    + simpl.
+      destruct (PT2IRT T1); trivial.
+
+   - simpl. destruct (string_dec var s); subst; simpl.
+     + tagOf2T.
+       replace (Pall2Lir (s |=> p; (s |=> Tvar; Γ)) e2)
+         with (Pall2Lir (s |=> p; Γ) e2); trivial.
+       eauto using Pall2LirEEnv,  inclusion_shadow,
+         PinclusionType, inclusion_shadow'.
+     + destruct (PT2IRT p); subst.
+       * tagOf2T.
+         destruct t;
+         simpl;
+            f_equal;
+            f_equal;
+           destruct (string_dec var s); try easy;
+           destruct (PT2IRT p0); simpl;
+               f_equal;
+                    replace (Pall2Lir (s |=> p; (var |=> Tvar; Γ)) e2)
+                      with  (Pall2Lir (var |=> Tvar; (s |=> p; Γ)) e2);
+                    eauto using Pall2LirEEnv, inclusion_permute,
+                                   PinclusionType.
+      * simpl.
+        f_equal.
+        f_equal.
+        ** destruct (string_dec var s); easy.
+        ** tagOf2T.
+           destruct (PT2IRT p0); simpl;
+           f_equal;
+           replace (Pall2Lir (s |=> p; (var |=> Tvar; Γ)) e2)
+             with  (Pall2Lir (var |=> Tvar; (s |=> p; Γ)) e2);
+           eauto using Pall2LirEEnv, inclusion_permute, PinclusionType.
+
+  - simpl. tagOf2T.
+    destruct (PT2IRT te); subst; destruct (PT2IRT T1); subst; simpl;
+    try destruct (dec_Tag t t0); subst; eauto.
+Qed.
+
+
+Lemma PValueValue : forall e, PValue e -> Value (Pall2Lir MEmpty e).
+Proof.
+  intros * PV.
+  induction PV; simpl; eauto using Value.
+  destruct (tagOf MEmpty v); eauto using Value.
+Defined.
+
+
+Fixpoint MPall2Lir (m : PMem) : Mem :=
+  match m with
+  | PEmptyMem => EmptyMem
+  | PUpdateT addr idx (PEV v ev) m =>
+      UpdateT addr
+              idx
+              (EV (Pall2Lir MEmpty v) (PValueValue v ev))
+              (MPall2Lir m)
+  | PUpdateF addr var T body m =>
+      UpdateF addr
+              var
+              (IRELet var (PT2IRT T) (<PT2IRT T <= IRTStar> (IREVar var))
+                 (Pall2Lir (var |=> T; MEmpty) body))
+              (MPall2Lir m)
+  end.
+
+
+Lemma MPall2LirCorrect : forall m,
+  Pmem_correct m -> mem_correct (MPall2Lir m).
+Proof.
+  induction m; intros H; only 1: constructor;
+  inversion H; subst.
+  - destruct p. eauto using mem_correct, Pall2LirWellTyped.
+  - constructor; auto.
+    constructor.
+    + eauto using inclusion_typing, inclusion_shadow', Pall2LirWellTyped.
+    + destruct (PT2IRT p); eauto using IRTyping, InEq.
+Qed.
+
+
+Lemma sameFreeaux : forall m,
+  Pfreshaux m = freshaux (MPall2Lir m).
+Proof.
+  induction m; trivial.
+  - destruct p. simpl. congruence.
+  - simpl. congruence.
+Qed.
+
+
+Lemma P2LfreshT : forall m m' free,
+  (free, m') = PfreshT m ->
+  (free, MPall2Lir m') = freshT (MPall2Lir m).
+Proof.
+  unfold PfreshT,  freshT.
+  intros * HEq.
+  induction m; injection HEq; intros; subst; trivial;
+  try (destruct p); rewrite sameFreeaux; trivial.
+Qed.
+
+
+Lemma TagFromType : forall e T,
+  MEmpty |= e : T ->
+  tagOf MEmpty e = PT2IRT T.
+Proof.
+  unfold tagOf. intros * HTy.
+  replace (typeOf MEmpty e) with (Some T); trivial.
+  symmetry; eauto using typeOfCorrect'.
+Qed.
+
+
+Lemma PreserveTagOf' : forall m e T m' e',
+  Pmem_correct m ->
+  m / e --> m' / e' ->
+  MEmpty |= e : T ->
+  tagOf MEmpty e' = PT2IRT T.
+Proof.
+  intros * HM HSt HTy.
+  eauto using TagFromType, PexpPreservation.
+Qed.
+
+
+Lemma PreserveTagOf : forall m e t m' e',
+  Pmem_correct m ->
+  MEmpty |= e : t ->
+  m / e --> m' / e' ->
+  tagOf MEmpty e = tagOf MEmpty e'.
+Proof.
+  unfold tagOf. intros * HM HTy Hst.
+  replace (typeOf MEmpty e') with (typeOf MEmpty e)
+        by eauto using pstep, PexpPreservTypeOf.
+  trivial.
+Qed.
+
+
+Lemma PqueryT2 : forall m a idx v,
+  Pmem_correct m ->
+  PqueryT a idx m = v ->
+  queryT a (IREBox TgInt (IRENum idx)) (MPall2Lir m) = Pall2Lir MEmpty v.
+Proof.
+  intros * HMC HQr.
+  generalize dependent v.
+  induction HMC; intros * HEq.
+  - simpl in HEq. subst. trivial.
+  - destruct v.
+    breakIndexDec; subst; simpl;
+    breakIndexDec; subst; simpl;
+      auto;
+      exfalso; auto.
+  - simpl. inversion HMC; subst; auto.
+Qed.
+
+
+Lemma PqueryF2 : forall m a var T body body',
+  Pmem_correct m ->
+  (var, T, body) = PqueryF a m ->
+  (var, body') = queryF a (MPall2Lir m) ->
+  body'= IRELet var (PT2IRT T) (< PT2IRT T <= IRTStar > IREVar var)
+               (Pall2Lir (var |=> T; MEmpty) body).
+Proof.
+  intros * HMC.
+  induction m; intros * HQr1 HQr2; inversion HMC; subst.
+  - injection HQr1; injection HQr2; intros; subst; trivial.
+  - destruct p. eauto.
+  - simpl in *. destruct (Nat.eq_dec a a0); eauto.
+    injection HQr1; injection HQr2; intros; subst; trivial.
+Qed.
+
+
+Lemma PqueryF2V : forall m a var var' T body body',
+  Pmem_correct m ->
+  (var, T, body) = PqueryF a m ->
+  (var', body') = queryF a (MPall2Lir m) ->
+  var = var'.
+Proof.
+  intros * HMC.
+  induction m; intros * HQr1 HQr2; inversion HMC; subst.
+  - injection HQr1; injection HQr2; intros; subst; trivial.
+  - destruct p. eauto.
+  - simpl in *. destruct (Nat.eq_dec a a0); eauto.
+    injection HQr1; injection HQr2; intros; subst; trivial.
+Qed.
+
+
+Lemma PCast2Lir : forall e T1 T2 v,
+  MEmpty |= e : T1 ->
+  PValue e ->
+  PCast e T2 = Some v ->
+  Pall2Lir MEmpty v = < PT2IRT T2 <= PT2IRT T1> (Pall2Lir MEmpty e).
+Proof.
+Abort.
+
+
+Lemma PCastBox : forall v T v' t,
+  MEmpty |= v : PTStar ->
+  PValue v ->
+  PCast v T = Some v' ->
+  PT2IRT T = Tag2Type t ->
+  Pall2Lir MEmpty v = IREBox t (Pall2Lir MEmpty v').
+Proof.
+  intros * HTy HV HCst Heq.
+  assert (T <> PTStar) by (intros contra; subst; discriminate).
+  specialize (ValStar _ HV HTy) as [v'' [Heq' HV']]; subst.
+  simpl in *.
+  assert (HCst': PCast v'' T = Some v') by (destruct T; easy).
+  inversion HTy; subst.
+  clear HCst HV HTy.
+  generalize dependent T.
+  generalize dependent t.
+  generalize dependent T1.
+  induction HV'; intros * HTy * HEq HNEq HCst.
+
+  - destruct T; simpl in *; try discriminate.
+    injection HEq; injection HCst; intros; subst. trivial.
+
+  - destruct T; simpl in *; try discriminate.
+    injection HEq; injection HCst; intros; subst. trivial.
+
+  - destruct T0; simpl in *; try discriminate.
+    injection HEq; injection HCst; intros; subst. trivial.
+
+  - destruct T; simpl in *; try discriminate.
+    injection HEq; injection HCst; intros; subst. trivial.
+
+  - unfold tagOf.
+    replace (typeOf MEmpty (PECast v PTStar)) with (Some T1)
+      by (symmetry; eauto using typeOfCorrect').
+    inversion HTy; subst.
+    simpl.
+    eapply IHHV'; clear IHHV'; eauto.
+    subst. simpl in *.
+    destruct T; trivial; discriminate.
+Qed.
+
+
+Lemma subsCast : forall var e T,
+  lir.substitution var e (< T <= IRTStar > IREVar var) =
+  < T <= IRTStar > e.
+Proof.
+  intros.
+  destruct T; simpl;
+  destruct (string_dec var var); easy.
+Qed.
+
+
+Lemma PCast2Star : forall {v v' T tg},
+  PValue v ->
+  MEmpty |= v : T ->
+  PT2IRT T = Tag2Type tg ->
+  PCast v PTStar = Some v' ->
+  Pall2Lir MEmpty v' = IREBox tg (Pall2Lir MEmpty v).
+Proof.
+  intros * HV HTy HEq HCast.
+  specialize (PT2IRTag _ _ HEq) as ?.
+  assert (v' = PECast v PTStar).
+  { induction HV; simpl in *;
+  injection HCast; try congruence.
+  exfalso.
+  inversion HTy; subst; eauto. }
+  subst; simpl.
+  tagOf2T.
+  destruct T; only 1: easy;
+  inversion HEq; subst; trivial.
+Qed.
+
+
+Lemma PCast2NStar : forall {v v' tg1 T1 tg2 T2},
+  PValue v ->
+  PT2IRT T1 = Tag2Type tg1 ->
+  PT2IRT T2 = Tag2Type tg2 ->
+  MEmpty |= v : T1 ->
+  PCast v T2 = Some v' ->
+  tg1 = tg2.
+Proof.
+  intros * HV HEq1 HEq2 HTy HCst.
+  destruct T1; only 1: (exfalso; eapply PT2IRTag in HEq1; easy);
+  destruct T2; only 1: (exfalso; eapply PT2IRTag in HEq2; easy);
+  inversion HEq1; inversion HEq2; subst; trivial;
+  inversion HTy; subst; discriminate.
+Qed.
+
+
+Lemma castTags : forall v v' T1 T2 t,
+  PValue v ->
+  MEmpty |= v : T1 ->
+  PCast v T2 = Some v' ->
+  PT2IRT T1 = Tag2Type t ->
+  PT2IRT T2 = Tag2Type t ->
+  Pall2Lir MEmpty v = Pall2Lir MEmpty v'.
+Proof.
+  intros * HV HTy HCst HEq1 HEq2.
+  induction HV; inversion HTy; subst; inversion HEq1; subst;
+  destruct T2; try discriminate;
+  simpl in HCst; try congruence;
+  injection HCst; intros; subst; trivial.
+Qed.
+
+
+Lemma castStar : forall v v' T t,
+  PValue v ->
+  MEmpty |= v : T ->
+  PCast v PTStar = Some v' ->
+  PT2IRT T = Tag2Type t ->
+  IREBox t (Pall2Lir MEmpty v) = Pall2Lir MEmpty v'.
+Proof.
+  intros * HV HTy HCst HEq.
+  induction HV; inversion HTy; subst; inversion HEq; subst;
+  simpl in HCst;
+  injection HCst; intros; subst; trivial.
+Qed.
+
+
+Lemma castFStar : forall v v' T t,
+  PValue v ->
+  MEmpty |= v : PTStar ->
+  PCast v T = Some v' ->
+  PT2IRT T = Tag2Type t ->
+  (Pall2Lir MEmpty v) = IREBox t (Pall2Lir MEmpty v').
+Proof.
+  intros * HV HTy HCst HEq.
+  induction HV; inversion HTy; subst.
+  simpl.
+  tagOf2T.
+  assert (PCast v T = Some v') by (destruct T; easy).
+  destruct (PT2IRT T1) eqn:?.
+  - replace t with t0 by eauto using PCast2NStar.
+    f_equal.
+    destruct HV; simpl;
+    destruct T; try easy;
+      try (simpl in H; injection H; intros; subst; trivial);
+      inversion H1; subst; discriminate.
+  - replace T1 with PTStar in * by (symmetry; auto using PTStarB).
+    auto.
+Qed.
+
+
+
+Lemma SimPallLir : forall m e T m' e',
+  Pmem_correct m ->
+  MEmpty |= e : T ->
+  m / e --> m' / e' ->
+  multistep (MPall2Lir m) (Pall2Lir MEmpty e)
+            (MPall2Lir m') (Pall2Lir MEmpty e').
+Proof.
+  intros * HM HTy HSt.
+  generalize dependent T.
+  induction HSt; intros * HTy;
+  inversion HTy; subst;
+
+  (* instantiate induction hipothesis *)
+  try match goal with
+    | [H: Pmem_correct ?m -> forall _, PTyping MEmpty ?E _ -> _,
+       HM: Pmem_correct ?m,
+       HTy: PTyping MEmpty ?E _ |- _] =>
+      specialize (H HM _ HTy)
+  end;
+  try (simpl; eauto using step, multistep1, PValueValue, P2LfreshT,
+              CongPlus1, CongPlus2; fail).
+
+  - simpl. tagOf2T.
+    destruct (PT2IRT T);
+    eauto using CongGet1, CongUnbox.
+
+  - simpl. tagOf2T.
+    destruct (PT2IRT T);
+    eauto using CongUnbox, CongGet2, CongBox, PValueValue.
+
+  - simpl. tagOf2T.
+    destruct (PT2IRT T0) eqn:?.
+    + simpl.
+      inversion H3; subst.
+      eapply MStMStep.
+      eapply StUnbox1; eauto using step, Value.
+      unshelve erewrite (PqueryT2 _ _ _ _ _ eq_refl); trivial.
+      eapply multistep1.
+      erewrite (PCastBox);
+      eauto using step, PValueValue, CastValue, PMCValue, PMCTy.
+    + simpl.
+      inversion H3; subst.
+      replace T0 with PTStar in * by (destruct T0; easy).
+      clear T0 Heqi.
+      eapply MStMStep; eauto using step, Value.
+      unshelve erewrite (PqueryT2 _ _ _ _ _ eq_refl); trivial.
+      erewrite CastToItsType in H; eauto using PMCValue, PMCTy.
+      injection H; intros; subst.
+      constructor.
+
+  - destruct (tagOf MEmpty e3); eauto using CongSet1.
+
+  - destruct (tagOf MEmpty e3); eauto using CongSet2, CongBox, PValueValue.
+
+  - simpl. tagOf2T.
+    destruct (PT2IRT T0);
+      eapply CongSet3; eauto using CongBox, PValueValue, Value.
+
+ - eapply multistep1.
+   eapply StSet.
+   eauto using Value.
+
+  - eapply multistep1.
+    eapply StFun.
+    fold Pall2Lir.
+    unfold PfreshF in H.
+    injection H; intros; subst.
+    unfold freshF.
+    rewrite sameFreeaux. trivial.
+
+  - simpl. tagOf2T.
+    destruct (PT2IRT T);
+    eauto using CongUnbox, CongFunApp1.
+
+  - simpl.
+    tagOf2T.
+    destruct (PT2IRT T);
+      destruct (PT2IRT T1);
+      eauto using CongUnbox, CongFunApp2, PValueValue, CongBox.
+
+  - inversion H5; subst.
+    destruct (queryF a (MPall2Lir m)) eqn:?.
+    replace s with var in * by eauto using PqueryF2V.
+    specialize (PqueryF2 m a var type body i HM H0 (eq_sym Heqp)).
+    assert (MEmpty |= v' : type) by eauto using CastEqType.
+    specialize (PMCTyF _ _ _ _ _ MEmpty H0 HM) as HTy'.
+    intros; subst.
+    simpl.
+    erewrite tagOfT'; eauto.
+    erewrite tagOfT'; eauto.
+    erewrite tagOfT'; eauto using Psubst_typing.
+    simpl.
+    eapply CongCast.
+    destruct (PT2IRT T0) eqn:?.
+
+    + eapply MStMStep.
+      * eapply StFunapp.
+        ** eauto using Value, PValueValue.
+        ** symmetry. eauto.
+      * simpl. destruct (string_dec var var); try easy.
+        clear e.
+        rewrite subsCast.
+        destruct (PT2IRT type) eqn:?.
+
+        ** simpl.
+           replace t0 with t in * by eauto using PCast2NStar.
+           eapply MStMStep.
+           *** eauto using step, PValueValue.
+           *** erewrite Psubst.
+               eapply multistep1.
+               **** replace (Pall2Lir MEmpty v')
+                       with (Pall2Lir MEmpty v) by eauto using castTags.
+               eauto using step, PValueValue.
+               **** eapply HTy'.
+               **** eauto using CastEqType.
+
+        ** simpl.
+           replace type with PTStar in * by (symmetry; auto using PTStarB).
+           erewrite castStar; eauto.
+           erewrite Psubst.
+           eapply multistep1.
+           *** eauto using step, PValueValue,  CastValue, Value.
+           *** eapply HTy'.
+           *** trivial.
+
+    + replace T0 with PTStar in * by (symmetry; auto using PTStarB).
+      clear Heqi.
+      eapply MStMStep.
+      * eapply StFunapp.
+        ** eauto using Value, PValueValue.
+        ** symmetry. eauto.
+      * simpl. destruct (string_dec var var); try easy.
+        clear e.
+        rewrite subsCast.
+        destruct (PT2IRT type) eqn:?.
+
+        ** simpl.
+           erewrite Psubst.
+           2: { eauto. }
+           2: { eauto. }
+           replace (Pall2Lir MEmpty v) with
+                   (IREBox t (Pall2Lir MEmpty v')) by
+                      (symmetry; eauto using castFStar).
+           eapply MStMStep;
+           eauto using step, MStMStep, multistep1, CastValue, PValueValue.
+
+        ** simpl.
+           replace type with PTStar in * by (symmetry; auto using PTStarB).
+           replace v' with v.
+           2:{ specialize (CastToItsType PTStar v H H7).
+               congruence. }
+           erewrite Psubst; eauto using multistep1, step, PValueValue.
+
+  - simpl. tagOf2T. eauto using CongCast.
+
+  - simpl. tagOf2T.
+    destruct (PT2IRT T0) eqn:?; destruct (PT2IRT T1) eqn:?; simpl.
+    + replace t0 with t in * by (symmetry; eauto using PCast2NStar).
+      destruct (dec_Tag t t); try easy.
+      erewrite castTags; eauto using multistep.
+    + replace T1 with PTStar in * by (symmetry; eauto using PTStarB).
+      erewrite PCastBox; eauto using multistep1, step, PValueValue,
+                                     CastValue.
+    + replace T0 with PTStar in * by (symmetry; eauto using PTStarB).
+      erewrite <- PCast2Star; eauto using multistep.
+    + replace T0 with PTStar in * by (symmetry; eauto using PTStarB).
+      replace T1 with PTStar in * by (symmetry; eauto using PTStarB).
+      specialize (CastToItsType _ _ H H6) as ?.
+      replace v' with v by congruence.
+      constructor.
+Qed.
+
 
 
